src/lang/Time.v
@@ -8,7 +8,20 @@ Require Import DenseOrder.
 Require Import Basic.
 Require Import Event.
 
-Module Time := DenseOrder.
+Set Implicit Arguments.
+
+Module Time.
+  Include DenseOrder.
+
+  Lemma lt_le_lt a b c
+        (AB: lt a b)
+        (BC: le b c):
+    lt a c.
+  Proof.
+    apply le_lteq in BC. des; subst; auto.
+    etransitivity; eauto.
+  Qed.
+End Time.
 
 Module TimeSet := UsualSet Time.
 Module TimeFun := UsualFun Time.
